Immutable example mostly working

Test/extern-soundness-immutable/ExternalConcatList.cs
@@ -1,0 +1,24 @@
+namespace Collections {
+
+  class ConcatList: DafnyCollections.List {
+    readonly DafnyCollections.List left;
+    readonly DafnyCollections.List right;
+
+    public ConcatList(DafnyCollections.List left, DafnyCollections.List right) {
+      this.left = left;
+      this.right = right;
+    }
+
+    public ulong Length() {
+      return left.Length() + right.Length();
+    }
+    
+    public ulong Get(ulong i) {
+      if (i < left.Length()) {
+        return left.Get(i);
+      } else {
+        return right.Get(i - left.Length());
+      }
+    }
+  }
+}
