Test/extern-soundness-immutable/ExternalList.dfy
@@ -1,83 +1,55 @@
 include "./List.dfy"
 
-module ExternalCollections {
+module {:extern "DafnyCollections"} ExternalCollections {
 
   import opened Collections
 
-  trait {:extern} ExternalList {
-
-    // TODO-RS: It may be possible to avoid the duplicate definitions of
-    // Valid() and Repr if this trait could extend ExternallyValid itself
+  trait {:extern "List"} ExternalList {
     predicate Valid() 
-      reads this, Repr 
-      ensures Valid() ==> this in Repr
-    ghost var Repr: set<object>
 
     // TODO-RS: figure out how to enforce that this acts like a function
-    function method Length(): int 
+    function method Length(): uint64 
       requires Valid()
-      reads Repr
     
-    method Get(i: int) returns (res: int)
-      modifies Repr
-    
-    method Set(i: int, element: int)
-      modifies Repr
-    
-    method Add(element: int)
-      modifies Repr
+    method Get(i: uint64) returns (res: uint64)
+      requires Valid()
+      ensures Valid()
   }
 
+  type ValidList? = l: List? | l == null || l.Valid()
+  type ValidExternalList? = l: ExternalList? | l == null || l.Valid()
+  
   /*
    * Adapts a Dafny-internal List as an ExternalList
    */
   class AsExternalList extends ExternalList {
 
-    var wrapped: List
+    const wrapped: ValidList?
 
     constructor(wrapped: List) 
       requires wrapped.Valid()
       ensures Valid()
     {
       this.wrapped := wrapped;
-      this.Repr := {this} + wrapped.Repr;
     }
 
     predicate Valid() 
-      reads this, Repr 
-      ensures Valid() ==> this in Repr
     {
-      && wrapped in Repr
-      && Repr == {this} + wrapped.Repr
+      && wrapped != null
       && wrapped.Valid()
     }
 
-    function method Length(): int
+    function method Length(): uint64
       requires Valid()
-      reads Repr
     {
       wrapped.Length()
     }
     
-    method Get(i: int) returns (res: int)
+    method Get(i: uint64) returns (res: uint64)
     {
+      expect wrapped != null;
       expect 0 <= i < wrapped.Length();
       res := wrapped.Get(i);
-    }
-    
-    method Set(i: int, element: int)
-    {
-      expect 0 <= i < wrapped.Length();
-      expect 0 <= element;
-      wrapped.Set(i, element);
-    }
-    
-    method Add(element: int)
-      modifies Repr
-      ensures fresh(Repr - old(Repr))
-    {
-      expect 0 <= element;
-      wrapped.Add(element);
     }
   }
 
@@ -86,88 +58,46 @@ module ExternalCollections {
    */
   class AsList extends List {
 
-    var wrapped: ExternalList
+    const wrapped: ValidExternalList?
 
     constructor(wrapped: ExternalList) 
       requires wrapped.Valid()
       ensures Valid()
     {
       this.wrapped := wrapped;
-      this.Repr := {this} + wrapped.Repr;
     }
 
     predicate Valid()
-      reads this, Repr
-      ensures Valid() ==> this in Repr 
     {
-      && wrapped in Repr
-      && Repr == {this} + wrapped.Repr
-      && wrapped.Valid()
+      wrapped != null && wrapped.Valid()
     }
 
-    function method Length(): nat
+    function method Length(): uint64
       requires Valid()
-      reads this, Repr
-      ensures Length() == |values|
+      ensures Valid()
+      ensures |values| < twoToThe64 && Length() == |values| as uint64
     {
       var result := wrapped.Length();
+
       // TODO-RS: Ideally we would include `expect result >= 0;`, but
       // we can't currently do that in a function, even though we really want that in
       // the compiled version.
-      Axiom(result == |values|);
+      Axiom(|values| < twoToThe64);
+      Axiom(result == |values| as uint64);
       result
     }
     
-    method Get(i: int) returns (res: nat)
+    method Get(i: uint64) returns (res: uint64)
       requires Valid()
       requires 0 <= i < Length()
-      modifies Repr
-      decreases Repr
       ensures Valid()
       ensures Length() == old(Length())
       ensures res == values[i]
     {
-      var result := wrapped.Get(i);
-      expect 0 <= result;
-      res := result;
+      res := wrapped.Get(i);
       
       Axiom(Length() == old(Length()));
       Axiom(res == values[i]);
-    }
-    
-    method Set(i: int, element: nat)
-      requires Valid()
-      requires 0 <= i < Length()
-      decreases Repr
-      modifies Repr
-      ensures Valid()
-      ensures values == old(values[..i]) + [element] + old(values[i + 1..])
-      ensures fresh(Repr - old(Repr))
-    {
-      wrapped.Set(i, element);
-
-      // Presumably cheap sanity check. This will be a tradeoff on a per-operation basis.
-      var elementAfter := wrapped.Get(i);
-      expect elementAfter == element;
-
-      values := values[..i] + [element] + values[i + 1..];
-    }
-
-    method Add(element: nat)
-      requires Valid()
-      decreases Repr
-      modifies Repr
-      ensures Valid()
-      ensures values == old(values) + [element]
-      ensures fresh(Repr - old(Repr))
-    {
-      var lengthBefore := Length();
-
-      wrapped.Add(element);
-
-      values := values + [element];
-
-      expect Length() == lengthBefore + 1;
     }
   }
 
