Test/extern-soundness-immutable/ListTest.dfy
@@ -1,15 +1,25 @@
-include "./ListUser.dfy"
+// RUN: %dafny /compile:3 /compileTarget:cs /print:"%t.print" /dprint:"%t.dprint" "%s" "%S%{dirsep}ExternalConcatList.cs" > "%t"
+// RUN: %diff "%s.expect" "%t"
+include "./ExternalList.dfy"
+include "./Math.dfy"
 
 module ListTest {
   import opened Collections
-  import opened ListUser
+  import opened Math
 
   method Main() {
-    var myList := new ArrayList();
-    myList.Add(1);
-    myList.Add(2);
-    myList.Add(3);
-    var sum := Sum(myList);
-    print "sum=", sum, "\n";
+    var list := new SequenceList([1, 2, 3, 4, 5]);
+    print "list.Length() = ", list.Length(), "\n";
+    
+    assert list.Length() == 5;
+    var result := list.Get(0);
+    print "list.Get(0) = ", result, "\n";
+    result := list.Get(2);
+    print "list.Get(2) = ", result, "\n";
+    result := list.Get(4);
+    print "list.Get(4) = ", result, "\n";
+
+    var sum := Sum(list);
+    print "Sum(list) = ", sum, "\n";
   }
 }
