Test/extern-soundness-immutable/Math.dfy
@@ -1,0 +1,35 @@
+include "./ExternalList.dfy"
+
+module Math {
+
+  import opened Collections
+  
+  method Sum(list: List) returns (res: int) 
+    requires list.Valid()
+  {
+    res := 0;
+    var i := 0;
+    var n := list.Length();
+    while i < n {
+      var element := list.Get(i);
+      res := res + element as int;
+      i := i + 1;
+    }
+  }
+}
+
+module {:extern "DafnyMath"} MathExtern {
+  import Math
+  import opened Collections
+  import opened ExternalCollections
+
+  // Exposed method for external client
+  method ExternalSum(list: ExternalList) returns (res: uint64)
+    requires list.Valid()
+  {
+    var asList := new AsList(list);
+    var result := Math.Sum(asList);
+    expect 0 <= result < twoToThe64;
+    res := result as uint64;
+  }
+}
